Add the transformer F

ltl/mu.v
@@ -1,12 +1,12 @@
 (*
  * mu-calculus for data words (of finite length)
  *)
-Require Import Nat Arith.
-Require Import List.
+Require Export Nat Arith.
+Require Export List.
 
 (* data words *)
 
-Parameter D : Set.  (* a data domain *)
+Definition D := nat.  (* a data domain *)
 Definition At := nat.  (* a finite set of atomic props *)
 Definition Sigma := At -> bool.  (* 2^{At} *)
 Definition data_word := list (Sigma * D)%type.
@@ -75,7 +75,7 @@ Definition update
   (theta : Theta) (i : register) (d : D) : Theta :=
   fun (r : register) => if r =? i then d else theta r.
 
-Definition Env := V -> list (data_word * Theta).
+Definition Env := V -> Theta -> data_word -> Prop.
 
 Definition models_atom
   (w : data_word) (theta : Theta) (atom : ltl_atom)
@@ -142,8 +142,8 @@ Inductive models :
        models u w' theta psi /\
        Forall_suffix_until (fun t => models_phi t theta phi) w' w) ->
       models u w theta (phi U psi)
-  | models_var : forall w theta u v,
-      In (w, theta) (u v) ->
+  | models_var : forall w theta (u : Env) v,
+      u v theta w ->
       models u w theta (var v)
   .
 
@@ -210,13 +210,154 @@ Axiom Theta_extensionality :
 Definition eqn_sys := V -> ltl.  (* the set of equation systems *)
 
 (* The transformation from Env to Env *)
-(*
 Definition F (eqns : eqn_sys) (env : Env) : Env :=
-*)
+  fun (v : V) (theta : Theta) (w : data_word) =>
+  (w, theta |= env, (eqns v)).
 
 (* the environment that assigns the empty set to every variable *)
 Definition empty_env : Env :=
-  fun (v : V) => nil.
+  fun (v : V) (theta : Theta) (w : data_word) => False.
+
+Section EqnExample.
+
+Variable b : Sigma.
+Local Definition w : data_word :=
+  ((b, 2) :: (b, 3) :: (b, 3) :: (b, 4) :: (b, 2) :: nil).
+Local Definition eqns : eqn_sys :=
+  fun v => match v with
+    1 => ↓ 1, X (var 2)
+  | 2 => ((X (var 2)) ./\ ~[↑ 1]) .\/ ((X (var 3)) ./\ [↑ 1])
+  | 3 => φ [END]
+  | _ => φ [tt]
+  end.
+
+Local Definition th : Theta :=
+  fun r => match r with
+    1 => 2
+  | _ => 0
+  end.
+
+Goal F eqns empty_env 3 th nil.
+Proof.
+  unfold F.
+  unfold eqns.
+  apply models_PHI.
+  unfold models_phi.
+  now unfold models_atom.
+Qed.
+Goal ~ F eqns empty_env 1 th nil.
+Proof.
+  unfold F.
+  unfold eqns.
+  intros H.
+  inversion H.
+Qed.
+Goal forall w' th',
+  ~ F eqns empty_env 1 th' w'.
+Proof.
+  intros w' th'.
+  unfold F.
+  unfold eqns.
+  intros H.
+  inversion H
+  as [| h t th'' u r psi Hht EQu EQht EQth'' [EQr EQpsi] | | | | | |].
+  clear th'' EQth'' u EQu r EQr psi EQpsi.
+  inversion Hht
+  as [| |h' t' th'' u psi Ht EQu [EQh' EQt'] EQth'' EQpsi| | | | |].
+  clear h' EQh' t' EQt' th'' EQth'' u EQu psi EQpsi.
+  inversion Ht
+  as [| | | | | | |w'' th'' u v He EQu EQw'' EQth'' EQv].
+  clear w'' EQw'' th'' EQth'' u EQu v EQv.
+  unfold empty_env in He.
+  contradiction.
+Qed.
+Goal forall w' th',
+  ~ F eqns empty_env 2 th' w'.
+Proof.
+  intros w' th'.
+  unfold F.
+  unfold eqns.
+  intros H.
+  inversion H
+  as [| | | | w'' th'' u psi1 psi2 Ho EQu EQw'' EQth'' [EQp1 EQp2]| | |].
+  clear w'' EQw'' th'' EQth'' u EQu psi1 EQp1 psi2 EQp2.
+  destruct Ho as [Ho | Ho].
+  - inversion Ho
+  as [| | |w'' th'' u psi phi Hx Hp EQu EQw'' EQth'' [EQpsi EQphi]| | | |].
+  clear w'' EQw'' th'' EQth'' u EQu psi EQpsi phi EQphi.
+  inversion Hx
+  as [| |h t th'' u psi Ht EQu EQht EQth'' EQpsi | | | | |].
+  clear th'' EQth'' u EQu psi EQpsi.
+  inversion Ht
+  as [| | | | | | |w'' th'' u v He EQu EQw'' EQth'' EQv].
+  clear w'' EQw'' th'' EQth'' u EQu v EQv.
+  unfold empty_env in He.
+  contradiction.
+  - inversion Ho
+  as [| | |w'' th'' u psi phi Hx Hp EQu EQw'' EQth'' [EQpsi EQphi]| | | |].
+  clear w'' EQw'' th'' EQth'' u EQu psi EQpsi phi EQphi.
+  inversion Hx
+  as [| |h t th'' u psi Ht EQu EQht EQth'' EQpsi | | | | |].
+  clear th'' EQth'' u EQu psi EQpsi.
+  inversion Ht
+  as [| | | | | | |w'' th'' u v He EQu EQw'' EQth'' EQv].
+  clear w'' EQw'' th'' EQth'' u EQu v EQv.
+  unfold empty_env in He.
+  contradiction.
+Qed.
+Goal (F eqns) ((F eqns) empty_env) 2 th ((b, 2)::nil).
+Proof.
+  unfold F.
+  unfold eqns at 2.
+  apply models_OR.
+  right.
+  apply models_AND.
+  - apply models_X.
+  apply models_var.
+  unfold eqns.
+  apply models_PHI.
+  unfold models_phi.
+  now unfold models_atom.
+  - unfold models_phi.
+  unfold models_atom.
+  unfold snd.
+  now unfold th.
+Qed.
+
+End EqnExample.
+
+Lemma meanings_of_models_var :
+  forall (w : data_word) (sigma : eqn_sys)
+    (theta : Theta) (u : Env) (v : V),
+  (w, theta |= F sigma u, var v) <->
+  (w, theta |= u, sigma v).
+Proof.
+  intros w sigma theta u v.
+  split.
+  - (* -> *)
+  intros H.
+  inversion H
+  as [| | | | | | |w' th u' v' H' EQu' EQw' EQth EQv'].
+  clear w' EQw' th EQth u' EQu' v' EQv'.
+  now unfold F in H'.
+  - (* <- *)
+  intros H.
+  apply models_var.
+  now unfold F.
+Qed.
+
+Lemma meanings_of_models_var_on_lfp :
+  forall (w : data_word) (sigma : eqn_sys)
+    (theta : Theta) (u : Env) (v : V),
+  u = F sigma u ->
+  (w, theta |= u, var v) <->
+  (w, theta |= u, sigma v).
+Proof.
+  intros w sigma theta u v.
+  intros Hlfp.
+  rewrite Hlfp at 1.
+  apply meanings_of_models_var.
+Qed.
 
 (* distribution over OR *)
 
